Memory.v
@@ -2,14 +2,91 @@ Import Nat.
 Require Import ZArith.
 
 
-Definition adr := nat.
+Parameter adr : Set.
 
-Definition Mem (T : Type) : Type := adr -> T.
+Parameter adr0 : adr.
+Parameter next : adr -> adr.
 
-Definition get {T} (r : adr) (m : Mem T) : T := m r.
+Fixpoint nextN (n : nat) (r : adr) : adr :=
+  match n with
+  | 0 => r
+  | S n' => next (nextN n' r)
+  end.
 
-Definition set {T} (r : adr) (v : T) (m : Mem T) : Mem T :=
-  fun r' => if eqb r r' then v else get r' m.
+Notation "r + n" := (nextN n r).
+
+Inductive lta (r : adr) : adr -> Prop :=
+| lea_self : lta r (next r)
+| lea_next r' : lta r r' -> lta r (next r').
+
+Hint Constructors lta.
+
+Infix "<" := lta.
+
+Definition lea r r' := r < r' \/ r = r'.
+
+Infix "<=" := lea.
+
+Axiom next_fresh : forall (r r' : adr), r < r' -> r <> r'.
+
+Parameter Mem : Type -> Type.
+
+Parameter get : forall {T}, adr -> Mem T -> T.
+Parameter set : forall {T}, adr -> T -> Mem T -> Mem T.
+
+Axiom get_set : forall T (r : adr) (v : T) (s :  Mem T), get r (set r v s) = v.
+Axiom get_get : forall T (r r' : adr) (v : T) (s :  Mem T), r <> r' -> get r (set r' v s) = get r s.
+
+Lemma lta_trans (r1 r2 r3 : adr) : r1 < r2 -> r2 < r3 -> r1 < r3.
+Proof.
+  intros R1 R2. induction R2;auto.
+Qed.
+
+Hint Resolve lta_trans.
+
+Lemma next_nextN r n : next (r + n) = next r + n.
+Proof.
+  generalize dependent r. induction n. reflexivity.
+  intros. simpl. rewrite IHn. reflexivity.
+Qed.
+
+Lemma lta_nextN r n : r < r + (S n).
+Proof.
+  induction n;simpl in *; auto.
+Qed.
+
+Lemma lta_next_eq (r r' : adr) : r < r' <-> exists n, r' = r + (S n).
+Proof.
+  split;intros.
+  - induction H.
+    + exists 0. reflexivity.
+    + destruct IHlta. exists (S x). simpl in *. subst. reflexivity.
+  - destruct H. subst. apply lta_nextN.
+Qed. 
+
+Lemma lea_lta r1 r2 r3 : r1 <= r2 -> r2 < r3 -> r1 < r3.
+Proof.
+  intros R1 R2. destruct R1. eauto. subst. assumption.
+Qed. 
+
+
+Lemma lta_lea r1 r2 r3 : r1 < r2 -> r2 <= r3 -> r1 < r3.
+Proof.
+  intros R1 R2. destruct R2. eauto. subst. assumption.
+Qed.
+
+Lemma lea_refl r : r <= r.
+Proof. unfold lea. auto. Qed.
+
+Lemma lea_sym r1 r2 r3 : r1 <= r2 -> r2 <= r3 -> r1 <= r3.
+Proof.
+  intros R1 R2.
+  destruct R1;subst;try assumption.
+  destruct R2; subst;try (left; assumption).
+  left. eauto.
+Qed. 
+
+Hint Resolve lta_lea lea_lta lea_sym lea_refl.
 
 Definition Eqr {T} (r : adr) (m1 m2 : Mem T) :=
   forall i : adr, i < r -> get i m1 = get i m2.
@@ -20,6 +97,8 @@ Notation "x =[ r ] y" := (Eqr r x y) (at level 70).
 Lemma eqr_refl T (x : Mem T) r : x =[ r ] x.
 Proof. intros i H. reflexivity. Qed.
 
+Hint Resolve eqr_refl.
+
 Lemma eqr_sym T (x y : Mem T) r : x =[ r ] y -> y =[ r ] x.
 Proof. intros R i E. apply R in E. auto. Qed.
 
@@ -29,37 +108,91 @@ Proof.
   rewrite E1. auto.
 Qed. 
 
-Lemma eqr_less T (x y : Mem T) r r' : x =[ r ] y -> r' <= r -> x =[ r' ] y.
-Proof. intros R L i L'. apply R. omega. Qed.
+Lemma eqr_lea T (x y : Mem T) r r' : x =[ r ] y -> r' <= r -> x =[ r' ] y.
+Proof. intros R L i L'. apply R. eauto. Qed.
 
+Lemma eqr_lta T (x y : Mem T) r r' : x =[ r ] y -> r' < r -> x =[ r' ] y.
+Proof. intros R L i L'. apply R. eauto. Qed.
 
-Lemma set_get_neq T r i (s : Mem T) n : r <> i -> get i s = get i (set r n s).
-Proof.
-  intro E. unfold get, set. remember (r =? i) as t. destruct t.
-  - rewrite <- Nat.eqb_neq in *. rewrite E in *. inversion Heqt.
-  - reflexivity.
-Qed.
 
 Lemma set_eqr T n (s s' : Mem T) r r' : set r n s =[r'] s' -> r < r' -> s =[r] s'.
 Proof.
-  intros H R i E. assert (i < r') as E' by omega. apply H in E'. rewrite <- E'.
-  apply set_get_neq. omega.
+  intros H R i E. assert (i < r') as E' by eauto. apply H in E'. rewrite <- E'.
+  symmetry. eauto using get_get, next_fresh.
 Qed.
 
-
-Lemma set_get T r (s : Mem T) n : get r (set r n s) = n.
-Proof.
-  unfold get, set. rewrite <- beq_nat_refl. reflexivity.
-Qed.
 
 Lemma set_get_eqr T r r' (s s' : Mem T) n : set r n s =[r'] s' -> r < r' -> get r s' = n.
 Proof.
-  intros R E. apply R in E. rewrite <- E. apply set_get.
+  intros R E. apply R in E. rewrite <- E. apply get_set.
+Qed.
+
+Lemma eqr_set  T r r' (s: Mem T) n : r <= r' -> set r' n s =[r] s.
+Proof.
+  unfold Eqr. intros R i I. apply get_get. apply next_fresh. eauto.
+Qed. 
+
+
+Definition rProp {T} (r: adr) (P : Mem T -> Prop) : Prop := forall s s', s =[r] s' -> (P s <-> P s').
+
+
+Ltac rProp_log := unfold rProp; intros Pr Qr s s' E;
+  pose (Pr s s' E) as Pr'; pose (Qr s s' E) as Qr';
+  rewrite Pr'; rewrite Qr'; tauto.
+
+Lemma rProp_conj r T (P Q : Mem T -> Prop) : rProp r P -> rProp r Q -> rProp r (fun s => P s /\ Q s).
+Proof. rProp_log. Qed. 
+
+Lemma rProp_disj r T (P Q : Mem T -> Prop) : rProp r P -> rProp r Q -> rProp r (fun s => P s \/ Q s).
+Proof. rProp_log. Qed.
+
+Lemma rProp_impl r T (P Q : Mem T -> Prop) : rProp r P -> rProp r Q -> rProp r (fun s => P s -> Q s).
+Proof. rProp_log. Qed.
+
+Lemma rProp_ex r T S (P : S -> Mem T -> Prop) : (forall a, rProp r (P a)) -> rProp r (fun s => exists a, P a s).
+Proof.
+  unfold rProp; intros Pr s s' E.
+  split; intros; destruct H; eexists.
+  rewrite <- Pr; eauto.
+  rewrite -> Pr; eauto.
+Qed.
+
+Lemma rProp_const T r P : rProp r (fun s : Mem T => P).
+Proof.
+  unfold rProp. tauto.
+Qed.
+
+Lemma rProp_get T r r' (v : T) : r' < r -> rProp r (fun s => get r' s = v).
+Proof.
+  unfold rProp. intros R s s' E. rewrite E. tauto. eauto.
+Qed.
+
+Lemma rProp_eqr T r (s' : Mem T) : rProp r (fun s => s' =[r] s).
+Proof.
+  unfold rProp. intros s1 s2 E. split; eauto using eqr_sym, eqr_trans. 
 Qed.
 
 
-Lemma set_eqr_incr T r (s s' : Mem T) n : s =[r] s' -> set r n s =[r + 1] set r n s'.
+Lemma rProp_lea T r r' (P : Mem T -> Prop) : r < r' -> rProp r P -> rProp r' P.
 Proof.
-  admit.
-Admitted.
+  unfold rProp. intros R Pr s s' E. eapply Pr. eauto using eqr_lta.
+Qed .
 
+Lemma rProp_ext T r (P : Mem T -> Prop) : rProp r P -> rProp r (fun s => P s).
+Proof. auto. Qed.
+
+Hint Resolve rProp_conj rProp_disj rProp_impl rProp_ex rProp_get rProp_lea rProp_ext rProp_const.
+
+Lemma rProp_set T (P : Mem T -> Prop) v s r r' : rProp r P -> r <= r' -> (P s <-> P (set r' v s)).
+Proof.
+  unfold rProp. intros Pr R. split;intro Ps; rewrite <- Pr; eauto using eqr_sym, eqr_set.
+Qed.
+
+Lemma rProp_set_r T (P : Mem T -> Prop) v s r: rProp r P -> P s -> P (set r v s).
+Proof. intros. rewrite <- rProp_set; eauto. Qed.
+
+Lemma rProp_set_l T (P : Mem T -> Prop) v s r : rProp r P -> P (set r v s) -> P s.
+Proof. intros. rewrite <- rProp_set in *; eauto. Qed.
+
+
+Ltac rProp_set_solve := eauto;try (rewrite <- rProp_set; eauto).
